impl spilling

theories/Spilling.v
@@ -1,5 +1,13 @@
 Require Import List Map Env AllInRel Exp MoreExp.
 Require Import IL Annotation InRel AutoIndTac Liveness.
+Require Import Bisim BisimTactics.
+
+
+Inductive stmt : Type :=
+ | stmtLet : var -> exp -> stmt -> stmt
+ | stmtReturn : exp -> stmt
+ | stmtIf : exp -> stmt -> stmt -> stmt.
+
 
 (* TODO: Read IL/Annotation.v which defines annotations for programs
          and figure out which type X to choose such that ann X is
@@ -10,9 +18,93 @@ Require Import IL Annotation InRel AutoIndTac Liveness.
          annotation and produces the spilled program
          assume a function [slot : var -> var] that yields the spill
          slot for a given variable *)
+Fixpoint write_spills (slot: var->var) (xs:list var) (s:stmt) : stmt :=
+match xs with
+| nil => s
+| x::xs => stmtLet (slot x) (Var x) (write_spills slot xs s) 
+end.
+
+Fixpoint write_loads (slot: var-> var) (xs:list var) (s:stmt) : stmt :=
+match xs with
+| nil => s
+| x::xs => stmtLet x (Var (slot x)) (write_loads slot xs s)
+end.
+
+
+Fixpoint doSpill (slot: var -> var) (s:stmt) (a:ann (set var * set var)) : stmt :=
+match s, a with
+| stmtLet x e s, ann1 (Sp,L) a =>
+    write_spills slot (to_list Sp)
+                 (write_loads slot (to_list L) (stmtLet x e (doSpill slot s a)))
+| _,_ => s
+end.
 
 (* TODO: read Liveness.v and figure out the type of the correctness
          predicate for spilling *)
+Inductive spill_sound : nat -> (list (set var * set var)) -> (set var * set var) -> stmt -> ann (set var * set var) -> Prop :=
+| SpillLet k Λ R M Sp L K Kx sl x e s
+: spill_sound k Λ ({x;(R\K ∪ L)\Kx }, M ∪ Sp) s sl
+->Exp.freeVars e ⊆ R\K ∪ L
+->cardinal (R\K ∪ L) <= k
+->cardinal ({x;((R\K) ∪ L)\Kx }) <= k
+->spill_sound k Λ (R,M) (stmtLet x e s) (ann1 (Sp,L) sl)
+| SpillReturn k Λ R M Sp L K e
+: Exp.freeVars e ⊆ R\K ∪ L
+ -> cardinal ((R\K) ∪ L) <= k
+ ->spill_sound k Λ (R,M) (stmtReturn e) (ann0 (Sp,L))
+| SpillIf k Λ R M Sp L K sl_s sl_t e s t
+: Exp.freeVars e ⊆ R\K ∪ L
+ -> cardinal (R\K ∪ L) <= k
+ -> spill_sound k Λ (R\K ∪ L, M ∪ Sp) s sl_s
+ -> spill_sound k Λ (R\K ∪ L, M ∪ Sp) t sl_t
+ -> spill_sound k Λ (R,M) (stmtIf e s t) (ann2 (Sp,L) sl_s sl_t)
+.
+
+Fixpoint stupSpill (R : set var) (s : stmt) : ann (set var * set var) := 
+(*fix stSp (R : set var) (s : stmt) : ann (set var * set var) := *)
+match s with
+| stmtLet x e t => ann1 (R, Exp.freeVars e) (stupSpill ((Exp.freeVars e) ∪ singleton x) t)
+| stmtReturn e => ann0 (R, Exp.freeVars e)
+| stmtIf e t v => ann2 (R, Exp.freeVars e) (stupSpill (Exp.freeVars e) t) (stupSpill (Exp.freeVars e) v)
+(*| stmtApp f xs => ann0 (R, ∅)*)
+(*| stmtFun f xs t v => ann2 (R, ∅) (stSp ∅ t) (stSp ∅ v)*)
+(*| _ => ann0 (∅,∅)*)
+end
+(*) ∅ s*)
+.
+
+Fixpoint freeVars (s:stmt) : set var :=
+  match s with
+    | stmtLet x e s0 => (freeVars s0 \ singleton x) ∪ Exp.freeVars e
+    | stmtIf e s1 s2 => freeVars s1 ∪ freeVars s2 ∪ Exp.freeVars e
+    | stmtReturn e => Exp.freeVars e
+  end.
+
+Set Implicit Arguments.
+Unset Strict Implicit.
+
+Lemma stupSpill_sat_spillSound (k:nat) (s:stmt) :
+(* forall e : exp in s, cardinal (Exp.freeVars) <= k*)
+freeVars s =  ∅ -> 
+spill_sound k nil (∅,∅) s (stupSpill ∅ s).
+assert (forall R M, freeVars s ⊆ R ∪ M -> spill_sound k nil (R,M) s (stupSpill R s)).
+ - intros R M subs.
+   induction s.
+   + simpl. simpl in subs. admit.
+   + admit.
+   + admit.
+ - intros. apply (H ∅ ∅). rewrite H0. admit.
+
+
+ destruct. assert (exists K, K ⊆ R /\ cardinal K = cardinal (Exp.freeVars e)).
+
+
+
+Theorem spill_sound_correct L E E' : spill_sound k Lsl (R,M) s alv asl
+-> (forall x : var, In x R -> E x = E' x)
+-> (forall x : var, In x S -> E x = E' (slot x))
+-> bisim (L,E,s) (L,E', doSpill slot s asl).
+
 
 (* TODO: define spilling predicate similarily to the liveness predicate
          in Liveness.v *)
